theories/LogicalRelation/Irrelevance.v
@@ -61,6 +61,8 @@ Context {wl Γ lA A lA' A'}
   (domRed' := (@PiRedTyPack.domRed _ _ _ _ _ _ _ _ _ _ _ _ _ _ _ _ _ ΠA'))
   (codomN := @PiRedTyPack.codomN _ _ _ _ _ _ _ _ _ _ _ _ _ _ _ _ _ ΠA)
   (codomN' := @PiRedTyPack.codomN _ _ _ _ _ _ _ _ _ _ _ _ _ _ _ _ _ ΠA')
+  (codomN_Ltrans := @PiRedTyPack.codomN_Ltrans _ _ _ _ _ _ _ _ _ _ _ _ _ _ _ _ _ ΠA)
+  (codomN_Ltrans' := @PiRedTyPack.codomN_Ltrans _ _ _ _ _ _ _ _ _ _ _ _ _ _ _ _ _ ΠA')
   (codRed := (@PiRedTyPack.codRed _ _ _ _ _ _ _ _ _ _ _ _ _ _ _ _ _ ΠA))
   (codRed' := (@PiRedTyPack.codRed  _ _ _ _ _ _ _ _ _ _ _ _ _ _ _ _ _ ΠA'))
   (eqPi : [Γ |- PiRedTyPack.prod ΠA ≅ PiRedTyPack.prod ΠA']< wl >).
@@ -68,31 +70,48 @@ Context {wl Γ lA A lA' A'}
 Context
   (eqvDomN : nat)
   (eqvDom : forall {Δ wl'} (ρ : Δ ≤ Γ) (τ : wl' ≤ε wl)
-                   (Ninfl : domN <= length wl')
-                   (Ninfl' : domN' <= length wl')
-                   (Ninfl'' : eqvDomN <= length wl')
+                   (Ninfl : AllInLCon domN wl')
+                   (Ninfl' : AllInLCon domN' wl')
+                   (Ninfl'' : AllInLCon eqvDomN wl')
                    (wfΔ : [  |- Δ]< wl' >),
       equivLRPack@{k k' v} (domRed Δ wl' ρ τ Ninfl wfΔ)
         (domRed' Δ wl' ρ τ Ninfl' wfΔ))
   (eqvCodN : forall {Δ a wl'} (ρ : Δ ≤ Γ) (τ : wl' ≤ε wl)
-                   (Ninfl : domN <= length wl')
-                   (Ninfl' : domN' <= length wl')
-                   (Ninfl'' : eqvDomN <= length wl')
+                   (Ninfl : AllInLCon domN wl')
+                   (Ninfl' : AllInLCon domN' wl')
+                   (Ninfl'' : AllInLCon eqvDomN wl')
                    (wfΔ : [  |- Δ]< wl' >)
           (ha : [domRed Δ wl' ρ τ Ninfl wfΔ| Δ ||- a : _]< wl' >)
           (ha' : [domRed' Δ wl' ρ τ Ninfl' wfΔ | Δ ||- a : _]< wl' >),
       nat)
+  (eqvCodN_Ltrans : forall {Δ a wl' wl''} (ρ : Δ ≤ Γ)
+                   (τ : wl' ≤ε wl) (τ' : wl'' ≤ε wl)
+                   (Ninfl : AllInLCon domN wl')
+                   (Ninfl' : AllInLCon domN wl'')
+                   (Minfl : AllInLCon domN' wl')
+                   (Minfl' : AllInLCon domN' wl'')
+                   (Kinfl : AllInLCon eqvDomN wl')
+                   (Kinfl' : AllInLCon eqvDomN wl'')
+                   (wfΔ : [  |- Δ]< wl' >)
+                   (wfΔ' : [  |- Δ]< wl'' >)
+          (ha : [domRed Δ wl' ρ τ Ninfl wfΔ| Δ ||- a : _]< wl' >)
+          (ha' : [domRed Δ wl'' ρ τ' Ninfl' wfΔ' | Δ ||- a : _]< wl'' >)
+          (ha2 : [domRed' Δ wl' ρ τ Minfl wfΔ| Δ ||- a : _]< wl' >)
+          (ha2' : [domRed' Δ wl'' ρ τ' Minfl' wfΔ' | Δ ||- a : _]< wl'' >),
+       wl'' ≤ε wl' ->
+      (eqvCodN ρ τ' Ninfl' Minfl' Kinfl' wfΔ' ha' ha2') <=
+        (eqvCodN ρ τ Ninfl Minfl Kinfl wfΔ ha ha2))
    (eqvCod : forall {Δ a wl'} (ρ : Δ ≤ Γ) (τ : wl' ≤ε wl)
-                    (Ninfl : domN <= length wl')
-                    (Ninfl' : domN' <= length wl')
-                    (Ninfl'' : eqvDomN <= length wl')
+                    (Ninfl : AllInLCon domN wl')
+                    (Ninfl' : AllInLCon domN' wl')
+                    (Ninfl'' : AllInLCon eqvDomN wl')
                     (wfΔ : [  |- Δ]< wl' >)
                     (ha : [domRed Δ wl' ρ τ Ninfl wfΔ| Δ ||- a : _]< wl' >)
                     (ha' : [domRed' Δ wl' ρ τ Ninfl' wfΔ | Δ ||- a : _]< wl' >)
                     {wl''} (τ' : wl'' ≤ε wl')
-                    (Minfl : codomN _ _ _ ρ τ Ninfl wfΔ ha <= length wl'')
-                    (Minfl' : codomN' _ _ _ ρ τ Ninfl' wfΔ ha' <= length wl'')
-                    (Minfl'' : eqvCodN ρ τ Ninfl Ninfl' Ninfl'' wfΔ ha ha' <= length wl''),
+                    (Minfl : AllInLCon (codomN _ _ _ ρ τ Ninfl wfΔ ha) wl'')
+                    (Minfl' : AllInLCon (codomN' _ _ _ ρ τ Ninfl' wfΔ ha') wl'')
+                    (Minfl'' : AllInLCon (eqvCodN ρ τ Ninfl Ninfl' Ninfl'' wfΔ ha ha') wl''),
        equivLRPack@{k k' v} (codRed Δ a wl' ρ τ Ninfl wfΔ ha wl'' τ' Minfl)
               (codRed' Δ a wl' ρ τ Ninfl' wfΔ ha' wl'' τ' Minfl')).
 
@@ -105,48 +124,72 @@ Proof.
   - intros ; cbn in *.
     unshelve eapply (max (max _ _) _).
     + unshelve eapply (codomN Δ a l' ρ τ _ h).
+      eapply AllInLCon_le ; try eassumption.
       eapply Nat.max_lub_r.
       now eapply Nat.max_lub_l.
       unshelve eapply eqvDom ; try assumption.
+      eapply AllInLCon_le ; try eassumption.
       now eapply Nat.max_lub_r.
     + unshelve eapply (codomN0 Δ a l' ρ τ _ _) ; try assumption.
-      * eapply Nat.max_lub_r.
+      * eapply AllInLCon_le ; try eassumption.
+        eapply Nat.max_lub_r.
         now eapply Nat.max_lub_l.
-      * eapply Nat.max_lub_l.
+      * eapply AllInLCon_le ; try eassumption.
+        eapply Nat.max_lub_l.
         now eapply Nat.max_lub_l.
       * unshelve  eapply eqvDom ; try assumption.
+        eapply AllInLCon_le ; try eassumption.
         now eapply Nat.max_lub_r.
     + unshelve eapply (eqvCodN Δ a l' ρ τ _ _ _) ; try assumption.
-      * eapply Nat.max_lub_r.
+      * eapply AllInLCon_le ; try eassumption.
+        eapply Nat.max_lub_r.
         now eapply Nat.max_lub_l.
-      * now eapply Nat.max_lub_r.
+      * eapply AllInLCon_le ; try eassumption.
+        now eapply Nat.max_lub_r.
       * unshelve eapply eqvDom ; try assumption.
+        eapply AllInLCon_le ; try eassumption.
         now eapply Nat.max_lub_r.
   - assumption.
   - cbn; etransitivity; [|tea]; now symmetry.
   - intros.
-    unshelve eapply eqvDom ; try eapply PeanoNat.Nat.max_lub_r ; try now eapply PeanoNat.Nat.max_lub_l.
-    eassumption.
-    unshelve eapply domRed0.
-    eapply Nat.max_lub_l.
-    now eapply Nat.max_lub_l.
-  - intros; cbn in *.
-    unshelve eapply eqvCod ; cbn in *.
-    + eapply Nat.max_lub_r.
+    unshelve eapply eqvDom ; try eapply AllInLCon_le ; try eassumption.
+    + eapply PeanoNat.Nat.max_lub_r ; now eapply PeanoNat.Nat.max_lub_l.
+    + now eapply PeanoNat.Nat.max_lub_r.      
+    + unshelve eapply domRed0.
+      eapply AllInLCon_le.
+      eapply Nat.max_lub_l.
       now eapply Nat.max_lub_l.
-    + now eapply Nat.max_lub_r.
-    + cbn in *.
-      unshelve eapply eqvDom ; try assumption.
+      eassumption.
+  - intros. cbn in *.
+    unshelve eapply Nat.max_le_compat.
+    + unshelve eapply Nat.max_le_compat.
+      * now eapply codomN_Ltrans.
+      * now eapply codomN_Ltrans0.
+    + now eapply eqvCodN_Ltrans.
+  - intros ; cbn in *.
+    unshelve eapply eqvCod ; cbn in *.
+    + eapply AllInLCon_le ; try eassumption.
+      eapply Nat.max_lub_r.
+      now eapply Nat.max_lub_l.
+    + eapply AllInLCon_le ; try eassumption.
       now eapply Nat.max_lub_r.
     + cbn in *.
+      unshelve eapply eqvDom ; try assumption.
+      eapply AllInLCon_le ; try eassumption.
+      now eapply Nat.max_lub_r.
+    + cbn in *.
+      eapply AllInLCon_le ; try eassumption.
       eapply Nat.max_lub_l.
       now eapply Nat.max_lub_l.
     + cbn in *.
+      eapply AllInLCon_le ; try eassumption.
       now eapply Nat.max_lub_r.
     + unshelve eapply codRed0.
-      * eapply Nat.max_lub_l.
+      * eapply AllInLCon_le ; try eassumption.
+        eapply Nat.max_lub_l.
         now eapply Nat.max_lub_l.
-      * eapply Nat.max_lub_r.
+      * eapply AllInLCon_le ; try eassumption.
+        eapply Nat.max_lub_r.
         now eapply Nat.max_lub_l.
 Qed.
 
@@ -158,49 +201,72 @@ Proof.
   - intros.
     unshelve refine (max (max _ _) _).
     + unshelve refine (appN Δ a l' ρ τ _ _ _ _) ; try assumption. 
-      * eapply Nat.max_lub_r.
+      * eapply AllInLCon_le ; try eassumption.
+        eapply Nat.max_lub_r.
         now eapply Nat.max_lub_l.
-      * eapply Nat.max_lub_l.
+      * eapply AllInLCon_le ; try eassumption.
+        eapply Nat.max_lub_l.
         now eapply Nat.max_lub_l.
       * unshelve eapply eqvDom ; try assumption.
+        eapply AllInLCon_le ; try eassumption.
         now eapply Nat.max_lub_r.
     + unshelve refine (codomN Δ a l' ρ τ _ _ _) ; try assumption. 
-      * eapply Nat.max_lub_r.
+      * eapply AllInLCon_le ; try eassumption.
+        eapply Nat.max_lub_r.
         now eapply Nat.max_lub_l.
       * unshelve eapply eqvDom ; try assumption.
+        eapply AllInLCon_le ; try eassumption.
         now eapply Nat.max_lub_r.
     + unshelve eapply (eqvCodN Δ a l' ρ τ _ _ _) ; try assumption.
-      * eapply Nat.max_lub_r.
+      * eapply AllInLCon_le ; try eassumption.
+        eapply Nat.max_lub_r.
         now eapply Nat.max_lub_l.
-      * now eapply Nat.max_lub_r.
+      * eapply AllInLCon_le ; try eassumption.
+        now eapply Nat.max_lub_r.
       * unshelve eapply eqvDom ; try assumption.
+        eapply AllInLCon_le ; try eassumption.
         now eapply Nat.max_lub_r.
   - now eapply redtmwf_conv.
   - assumption.
   - apply (tm_nf_conv isnf).
     + destruct ΠA'; simpl in * ; apply eqPi.
   - now eapply convtm_conv.
+  - intros ; cbn in *.
+    unshelve eapply Nat.max_le_compat.
+    + unshelve eapply Nat.max_le_compat.
+      * now eapply appN_Ltrans.
+      * now eapply codomN_Ltrans.
+    + now eapply eqvCodN_Ltrans.
   - intros; unshelve eapply eqvCod.
-    + eapply Nat.max_lub_r.
+    + eapply AllInLCon_le ; try eassumption.
+      eapply Nat.max_lub_r.
       now eapply Nat.max_lub_l.
-    + now eapply Nat.max_lub_r.
+    + eapply AllInLCon_le ; try eassumption.
+      now eapply Nat.max_lub_r.
     + cbn in *.
       unshelve eapply eqvDom ; try assumption.
+      eapply AllInLCon_le ; try eassumption.
       now eapply Nat.max_lub_r.
-    + eapply Nat.max_lub_r.
+    + eapply AllInLCon_le ; try eassumption.
+      eapply Nat.max_lub_r.
       now eapply Nat.max_lub_l.
-    + now eapply Nat.max_lub_r.
+    + eapply AllInLCon_le ; try eassumption.
+      now eapply Nat.max_lub_r.
     + cbn in *.
       eapply app.
+      eapply AllInLCon_le ; try eassumption.
       eapply Nat.max_lub_l.
       now eapply Nat.max_lub_l.
   - intros; unshelve eapply eqvCod, eq.
     all: try eapply eqvDom ; try eassumption.
-    all: try (eapply Nat.max_lub_r ;
+    all: try (eapply AllInLCon_le ; try eassumption ;
+              eapply Nat.max_lub_r ;
               now eapply Nat.max_lub_l).
-    all: try (eapply Nat.max_lub_l ;
+    all: try (eapply AllInLCon_le ; try eassumption ; 
+              eapply Nat.max_lub_l ;
               now eapply Nat.max_lub_l).
-    all: try now eapply Nat.max_lub_r.
+    all: try now eapply AllInLCon_le ; try eassumption ;
+      eapply Nat.max_lub_r.
 Defined.
 
 Lemma ΠIrrelevanceTmEq t u : [Γ ||-<lA> t ≅ u : A | RA]< wl > -> [Γ ||-<lA'> t ≅ u : A' | RA']< wl >.
@@ -211,31 +277,51 @@ Proof.
   - intros.
     unshelve refine (max (max _ _) _).
     + unshelve refine (eqappN Δ a l' ρ τ _ _ _ _) ; try assumption.
-      * eapply Nat.max_lub_r ; now eapply Nat.max_lub_l.
-      * eapply Nat.max_lub_l ; now eapply Nat.max_lub_l.
+      * eapply AllInLCon_le ; try eassumption.
+        eapply Nat.max_lub_r ; now eapply Nat.max_lub_l.
+      * eapply AllInLCon_le ; try eassumption.
+        eapply Nat.max_lub_l ; now eapply Nat.max_lub_l.
       * unshelve eapply eqvDom ; try assumption.
+        eapply AllInLCon_le ; try eassumption.
         now eapply Nat.max_lub_r.
     + unshelve refine (codomN Δ a l' ρ τ _ _ _) ; try assumption. 
-      * eapply Nat.max_lub_r ; now eapply Nat.max_lub_l.
+      * eapply AllInLCon_le ; try eassumption.
+        eapply Nat.max_lub_r ; now eapply Nat.max_lub_l.
       * unshelve eapply eqvDom ; try assumption.
+        eapply AllInLCon_le ; try eassumption.
         now eapply Nat.max_lub_r.
     + unshelve eapply (eqvCodN Δ a l' ρ τ _ _ _) ; try assumption.
-      * eapply Nat.max_lub_r.
+      * eapply AllInLCon_le ; try eassumption.
+        eapply Nat.max_lub_r.
         now eapply Nat.max_lub_l.
-      * now eapply Nat.max_lub_r.
+      * eapply AllInLCon_le ; try eassumption.
+        now eapply Nat.max_lub_r.
       * unshelve eapply eqvDom ; try assumption.
+        eapply AllInLCon_le ; try eassumption.
         now eapply Nat.max_lub_r.
   - now eapply convtm_conv.
+  - intros ; cbn in *.
+    unshelve eapply Nat.max_le_compat.
+    + unshelve eapply Nat.max_le_compat.
+      * now eapply eqappN_Ltrans.
+      * now eapply codomN_Ltrans.
+    + now eapply eqvCodN_Ltrans.
   - intros; unshelve eapply eqvCod.
-    + eapply Nat.max_lub_r ; now eapply Nat.max_lub_l.
-    + now eapply Nat.max_lub_r.
+    + eapply AllInLCon_le ; try eassumption.
+      eapply Nat.max_lub_r ; now eapply Nat.max_lub_l.
+    + eapply AllInLCon_le ; try eassumption.
+      now eapply Nat.max_lub_r.
     + cbn in *.
       unshelve eapply eqvDom ; try assumption.
+      eapply AllInLCon_le ; try eassumption.
       now eapply Nat.max_lub_r.
-    + eapply Nat.max_lub_r ; now eapply Nat.max_lub_l.
-    + now eapply Nat.max_lub_r.
+    + eapply AllInLCon_le ; try eassumption.
+      eapply Nat.max_lub_r ; now eapply Nat.max_lub_l.
+    + eapply AllInLCon_le ; try eassumption.
+      now eapply Nat.max_lub_r.
     + cbn in *.
       eapply eqApp.
+      eapply AllInLCon_le ; try eassumption.
       eapply Nat.max_lub_l ; now eapply Nat.max_lub_l.
 Qed.
 
@@ -253,36 +339,55 @@ Lemma ΠIrrelevanceLRPack@{i j k l i' j' k' l' v}
   (domRed' := (@PiRedTyPack.domRed _ _ _ _ _ _ _ _ _ _ _ _ _ _ _ _ _ ΠA'))
   (codomN := @PiRedTyPack.codomN _ _ _ _ _ _ _ _ _ _ _ _ _ _ _ _ _ ΠA)
   (codomN' := @PiRedTyPack.codomN _ _ _ _ _ _ _ _ _ _ _ _ _ _ _ _ _ ΠA')
+  (codomN_Ltrans := @PiRedTyPack.codomN_Ltrans _ _ _ _ _ _ _ _ _ _ _ _ _ _ _ _ _ ΠA)
+  (codomN_Ltrans' := @PiRedTyPack.codomN_Ltrans _ _ _ _ _ _ _ _ _ _ _ _ _ _ _ _ _ ΠA')
   (codRed := (@PiRedTyPack.codRed  _ _ _ _ _ _ _ _ _ _ _ _ _ _ _ _ _ ΠA))
   (codRed' := (@PiRedTyPack.codRed  _ _ _ _ _ _ _ _ _ _ _ _ _ _ _ _ _ ΠA'))
   (eqPi : [Γ |- PiRedTyPack.prod ΠA ≅ PiRedTyPack.prod ΠA']< wl >)
   (eqvDomN : nat)
   (eqvDom : forall {Δ wl'} (ρ : Δ ≤ Γ) (τ : wl' ≤ε wl)
-                   (Ninfl : domN <= length wl')
-                   (Ninfl' : domN' <= length wl')
-                   (Ninfl'' : eqvDomN <= length wl')
+                   (Ninfl : AllInLCon domN wl')
+                   (Ninfl' : AllInLCon domN' wl')
+                   (Ninfl'' : AllInLCon eqvDomN wl')
                    (wfΔ : [  |- Δ]< wl' >),
       equivLRPack@{k k' v} (domRed Δ wl' ρ τ Ninfl wfΔ)
         (domRed' Δ wl' ρ τ Ninfl' wfΔ))
   (eqvCodN : forall {Δ a wl'} (ρ : Δ ≤ Γ) (τ : wl' ≤ε wl)
-                   (Ninfl : domN <= length wl')
-                   (Ninfl' : domN' <= length wl')
-                   (Ninfl'' : eqvDomN <= length wl')
+                   (Ninfl : AllInLCon domN wl')
+                   (Ninfl' : AllInLCon domN' wl')
+                   (Ninfl'' : AllInLCon eqvDomN wl')
                    (wfΔ : [  |- Δ]< wl' >)
           (ha : [domRed Δ wl' ρ τ Ninfl wfΔ| Δ ||- a : _]< wl' >)
           (ha' : [domRed' Δ wl' ρ τ Ninfl' wfΔ | Δ ||- a : _]< wl' >),
       nat)
+  (eqvCodN_Ltrans : forall {Δ a wl' wl''} (ρ : Δ ≤ Γ)
+                   (τ : wl' ≤ε wl) (τ' : wl'' ≤ε wl)
+                   (Ninfl : AllInLCon domN wl')
+                   (Ninfl' : AllInLCon domN wl'')
+                   (Minfl : AllInLCon domN' wl')
+                   (Minfl' : AllInLCon domN' wl'')
+                   (Kinfl : AllInLCon eqvDomN wl')
+                   (Kinfl' : AllInLCon eqvDomN wl'')
+                   (wfΔ : [  |- Δ]< wl' >)
+                   (wfΔ' : [  |- Δ]< wl'' >)
+          (ha : [domRed Δ wl' ρ τ Ninfl wfΔ| Δ ||- a : _]< wl' >)
+          (ha' : [domRed Δ wl'' ρ τ' Ninfl' wfΔ' | Δ ||- a : _]< wl'' >)
+          (ha2 : [domRed' Δ wl' ρ τ Minfl wfΔ| Δ ||- a : _]< wl' >)
+          (ha2' : [domRed' Δ wl'' ρ τ' Minfl' wfΔ' | Δ ||- a : _]< wl'' >),
+      wl'' ≤ε wl' ->
+      (eqvCodN ρ τ' Ninfl' Minfl' Kinfl' wfΔ' ha' ha2') <=
+        (eqvCodN ρ τ Ninfl Minfl Kinfl wfΔ ha ha2))
    (eqvCod : forall {Δ a wl'} (ρ : Δ ≤ Γ) (τ : wl' ≤ε wl)
-                    (Ninfl : domN <= length wl')
-                    (Ninfl' : domN' <= length wl')
-                    (Ninfl'' : eqvDomN <= length wl')
+                    (Ninfl : AllInLCon domN wl')
+                    (Ninfl' : AllInLCon domN' wl')
+                    (Ninfl'' : AllInLCon eqvDomN wl')
                     (wfΔ : [  |- Δ]< wl' >)
                     (ha : [domRed Δ wl' ρ τ Ninfl wfΔ| Δ ||- a : _]< wl' >)
                     (ha' : [domRed' Δ wl' ρ τ Ninfl' wfΔ | Δ ||- a : _]< wl' >)
                     {wl''} (τ' : wl'' ≤ε wl')
-                    (Minfl : codomN _ _ _ ρ τ Ninfl wfΔ ha <= length wl'')
-                    (Minfl' : codomN' _ _ _ ρ τ Ninfl' wfΔ ha' <= length wl'')
-                    (Minfl'' : eqvCodN ρ τ Ninfl Ninfl' Ninfl'' wfΔ ha ha' <= length wl''),
+                    (Minfl : AllInLCon (codomN _ _ _ ρ τ Ninfl wfΔ ha) wl'')
+                    (Minfl' : AllInLCon (codomN' _ _ _ ρ τ Ninfl' wfΔ ha') wl'')
+                    (Minfl'' : AllInLCon (eqvCodN ρ τ Ninfl Ninfl' Ninfl'' wfΔ ha ha') wl''),
        equivLRPack@{k k' v} (codRed Δ a wl' ρ τ Ninfl wfΔ ha wl'' τ' Minfl)
          (codRed' Δ a wl' ρ τ Ninfl' wfΔ ha' wl'' τ' Minfl'))
    : equivLRPack@{k k' v} RA RA'.
@@ -539,7 +644,7 @@ Proof.
     destruct lrA' as [| | ? ? A' ΠA' HAad' | | |] ; try solve [destruct s] ; clear s.
     pose (PA := PiRedTyPack.pack ΠA HAad).
     pose (PA' := PiRedTyPack.pack ΠA' HAad').
-    destruct he as [dom0 cod0 ??? domRed ? codRed], ΠA' as [dom1 cod1].
+    destruct he as [dom0 cod0 ??? domRed ? ? codRed], ΠA' as [dom1 cod1].
     assert (tProd dom0 cod0 = tProd dom1 cod1) as ePi
     by (eapply whredty_det ; gen_typing).
     inversion ePi ; subst ; clear ePi.
@@ -551,6 +656,8 @@ Proof.
       intros; unshelve eapply IHdom.
       1: now eapply (LRAd.adequate (PiRedTyPack.domRed PA' _ _ _ _)).
       now eapply domRed.
+    + intros ; cbn in *.
+      now eapply codomN_Ltrans.
     + intros; unshelve eapply IHcod.
       1: eapply (LRAd.adequate (PiRedTyPack.codRed PA' _ _ _ _ _ _ _)).
       now eapply codRed. 
@@ -587,6 +694,8 @@ Proof.
     + intros Δ a wl' ρ τ Ninfl tΔ ra.
       now eapply IHcod.
     + assumption.
+    + cbn ; intros.
+      now eapply codomN_Ltrans.
     + cbn. intros Δ a b wl' ρ τ Ninfl tΔ ra rb rab wl'' τ' Minfl.
       destruct (LRIrrelevantPreds IH wl' Δ (dom⟨ρ⟩) (dom⟨ρ⟩)
                   (domAd  Δ wl' ρ τ Ninfl tΔ) (IHdom  Δ wl' ρ τ Ninfl tΔ : LRPackAdequate (LogRel@{i' j' k' l'} lA) (IHdom  Δ wl' ρ τ Ninfl tΔ))
@@ -704,8 +813,12 @@ Proof.
   intros.
   eapply LRTyEqIrrelevantCum.
   unshelve eapply WRedEq ; try assumption.
-  + now eapply Nat.max_lub_l.
-  + now eapply Nat.max_lub_r.
+  + eapply AllInLCon_le.
+    now eapply Nat.max_lub_l.
+    eassumption.
+  + eapply AllInLCon_le.
+    now eapply Nat.max_lub_r.
+    eassumption.
 Qed.
 
 Corollary RedTmIrrelevantCum wl Γ A {lA eqTyA redTmA eqTmA lA' eqTyA' redTmA' eqTmA'}
@@ -749,8 +862,12 @@ Proof.
   exists (max lrA.(WN) WNTm).
   intros ; eapply LRTmRedIrrelevantCum.
   unshelve eapply WRedTm ; try assumption.
-  + now eapply Nat.max_lub_l.
-  + now eapply Nat.max_lub_r.
+  + eapply AllInLCon_le.
+    now eapply Nat.max_lub_l.
+    eassumption.
+  + eapply AllInLCon_le.
+    now eapply Nat.max_lub_r.
+    eassumption.
 Qed.
 
 Corollary TmEqIrrelevantCum wl Γ A {lA eqTyA redTmA eqTmA lA' eqTyA' redTmA' eqTmA'}
@@ -794,8 +911,12 @@ Proof.
   exists (max lrA.(WN) WNTmEq).
   intros ; eapply LRTmEqIrrelevantCum.
   unshelve eapply WRedTmEq ; try assumption.
-  + now eapply Nat.max_lub_l.
-  + now eapply Nat.max_lub_r.
+  + eapply AllInLCon_le.
+    now eapply Nat.max_lub_l.
+    eassumption.
+  + eapply AllInLCon_le.
+    now eapply Nat.max_lub_r.
+    eassumption.
 Qed.
   
 
@@ -884,10 +1005,12 @@ Proof.
     symmetry; eassumption.
   - intros * ihdom ihcod * []. unshelve econstructor.
     1,2: eassumption.
-    assumption.
-    assumption.
-    1: symmetry; eassumption.
-    intros. apply ihcod. now eapply eqApp.
+    + assumption.
+    + assumption.
+    + symmetry; eassumption.
+    + cbn in * ; intros.
+      now eapply eqappN_Ltrans.
+    + intros. apply ihcod. now eapply eqApp.
   - intros ???? NA.
     set (G := _); enough (h : G × (forall t u, NatPropEq NA t u -> NatPropEq NA u t)) by apply h.
     subst G; apply NatRedEqInduction.
@@ -951,6 +1074,7 @@ Proof.
     + now eapply wft_Ltrans.
     + now eapply wft_Ltrans.
     + now eapply convty_Ltrans.
+    + cbn. intros ; now eapply codomN_Ltrans.
     + intros ; now eapply codExt.
     + cbn in *.
       econstructor.
@@ -1055,6 +1179,7 @@ Ltac irrelevance0 :=
 Ltac irrelevance := irrelevance0 ; [|eassumption] ; try first [reflexivity| now bsimpl].
 
 Ltac irrelevanceRefl := irrelevance0 ; [reflexivity|].
+
 
 
 Section IrrelevanceLCon.
