theories/LogicalRelation/NormalRed.v
@@ -72,21 +72,28 @@ Obligation 7.
   now irrelevance.
 Defined.
 Obligation 8.
+  destruct h as [??????? domRed codomN ? codRed codExt] ; 
+    intros; cbn in *.
+  now eapply codomN_Ltrans.
+Defined.
+
+Obligation 9.
   intros;
   assert (wΠ : whnf (tProd F G)) by constructor.
   pose proof (e := redtywf_whnf (PiRedTyPack.red h) wΠ).
   symmetry in e; injection e; clear e.
-  destruct h as [??????? domRed codomN codRed codExt] ; 
+  destruct h as [??????? domRed codomN ? codRed codExt] ; 
     intros; cbn in *.
   subst.
   unshelve eapply codRed ;[exact wl' |..] ; tea.
 Defined.
+
 Next Obligation.
   intros;
   assert (wΠ : whnf (tProd F G)) by constructor.
   pose proof (e := redtywf_whnf (PiRedTyPack.red h) wΠ).
   symmetry in e; injection e; clear e.
-  destruct h as [??????? domRed codomN codRed codExt] ; 
+  destruct h as [??????? domRed codomN ? codRed codExt] ; 
     intros; cbn in *.
   subst.
   irrelevance0 ; try reflexivity.
@@ -112,18 +119,18 @@ Obligation 6.
     destruct Rlam as [??????? app eqq]; cbn in *.
   unshelve eapply appN ; try eassumption ; subst ; try eassumption.
 Defined.
+Obligation 7.
+  intros;
+    destruct Rlam as  [???????? app eqq].
+  unshelve eapply appN_Ltrans ; try assumption.
+Defined.
 
 Solve All Obligations with
   intros;
   pose proof (e := redtmwf_whnf (PiRedTm.red Rlam) whnf_tLambda);
-  destruct Rlam as [??????? app eqq]; cbn in *; try exact redN ; subst;
-first [eapply app | now eapply eqq| eassumption].
-Next Obligation.
-  intros;
-  pose proof (e := redtmwf_whnf (PiRedTm.red Rlam) whnf_tLambda);
-    destruct Rlam as  [??????? app eqq]; cbn in *; subst.
-  unshelve eapply app ; try assumption.
-Defined.
+  destruct Rlam as [???????? app eqq]; cbn in *; try exact redN ; subst;
+first [eapply app ; eassumption | now eapply eqq| eassumption].
+  
 
 End Normalization.
 
